@prefix :     <http://goonmill.org/2007/characteristic.n3#> .
@prefix p:     <http://goonmill.org/2007/property.n3#> .
@prefix rdfs: <http://www.w3.org/2000/01/rdf-schema#> .

<> rdfs:title "Character Characteristics" .
<> rdfs:comment """Characteristics of creatures both PC and NPC
TODO - add much of this to perk.n3 as tags?
""" .


:Characteristic a rdfs:Class .


:MiscTrait rdfs:subClassOf :Characteristic;
    rdfs:comment "Aspect of a creature that does not fall into any other category.";
.

:ChallengeRating a rdfs:Class;
    rdfs:comment "The CR value for a monster, which may have annotations.";
.

:Race rdfs:subClassOf :Characteristic .

:Save rdfs:subClassOf :Characteristic .

:Fort rdfs:subClassOf :Save; rdfs:label "Fortitude" .
:Ref rdfs:subClassOf :Save; rdfs:label "Reflex" .
:Will rdfs:subClassOf :Save; rdfs:label "Will" .


:Family rdfs:subClassOf :Characteristic .


:Sense rdfs:subClassOf :Characteristic .

:Darkvision rdfs:subClassOf :Sense .

:Blindsense rdfs:subClassOf :Sense .



:Alignment rdfs:subClassOf :Characteristic .
:AlignmentAtom rdfs:subClassOf :Alignment.
:AlignmentTrue rdfs:subClassOf :Alignment;
    rdfs:comment "A complete moral-ethic alignment, those available to PCs";
.

:lawfulGood      a  :AlignmentTrue .
:neutralGood     a  :AlignmentTrue .
:chaoticGood     a  :AlignmentTrue .
:lawfulNeutral   a  :AlignmentTrue .
:neutralNeutral  a  :AlignmentTrue .
:chaoticNeutral  a  :AlignmentTrue .
:lawfulEvil      a  :AlignmentTrue .
:neutralEvil     a  :AlignmentTrue .
:chaoticEvil     a  :AlignmentTrue .
:noAlignment     a  :AlignmentTrue .
:lawful          a  :AlignmentAtom .
:chaotic         a  :AlignmentAtom .
:evil            a  :AlignmentAtom .
:good            a  :AlignmentAtom .
:neutralMorals   a  :AlignmentAtom .
:neutralEthics   a  :AlignmentAtom .


:AttackEffect rdfs:subClassOf :Characteristic .
:Energy rdfs:subClassOf :Characteristic .

:mindAffecting a :AttackEffect;
    rdfs:label "Mind-Affecting Attacks"
.
:acid a :AttackEffect, :Energy .
:cold a :AttackEffect, :Energy .
:fire a :AttackEffect, :Energy .
:electricity a :AttackEffect, :Energy .
:sonic a :AttackEffect, :Energy .
:poison a :AttackEffect .
:sleep a :AttackEffect .
:paralysis a :AttackEffect .
:polymorph a :AttackEffect .
:stunning a :AttackEffect .
:disease a :AttackEffect .
:deathEffects a :AttackEffect;
    rdfs:label "Death Effects";
.
:necromancy a :AttackEffect .
:petrification a :AttackEffect .
:nonMagical a :AttackEffect;
    rdfs:label "Non-Magical Attacks";
.
:piercing a :AttackEffect .
:slashing a :AttackEffect .
:areaEffect a :AttackEffect;
    rdfs:label "Area-Effect Attacks";
.
:magic a :AttackEffect;
    rdfs:comment "Damage from magical attacks";
.

:Resistance rdfs:subClassOf :MiscTrait.


:Perk rdfs:subClassOf :MiscTrait .

:Immunity rdfs:subClassOf :Characteristic .

:Vulnerability rdfs:subClassOf :Characteristic .

:Resistance rdfs:subClassOf :Characteristic .

:Language rdfs:subClassOf :Characteristic .


:SpecialQuality rdfs:subClassOf :MiscTrait .



:Proficiency rdfs:subClassOf :Characteristic .
:martialWeapons a :Proficiency; rdfs:label "Martial Weapons" .
:simpleWeapons a :Proficiency; rdfs:label "Simple Weapons" .
:naturalWeapons a :Proficiency; rdfs:label "Natural Weapons" .
:armorNone a :Proficiency; rdfs:label "Proficient with no armor" .
:weaponsAsDescribed a :Proficiency;
    rdfs:label "Proficient with whatever weapons are in its description";
    rdfs:comment "If generally humanoid in form, proficient with whatever weapons are in its description";
.
:armorAsDescribed a :Proficiency;
    rdfs:label "Proficient with whatever armor it is described as wearing";
    rdfs:comment "Proficient with whatever type of armor (light, medium, or heavy) that it is described as wearing, as well as all lighter types.  This creature, when not indicated as wearing armor is not proficient with armor. This creature is proficient with shields if it is proficient with any form of armor.";
.



:Vitality rdfs:subClassOf :Characteristic .



:CombatMechanic rdfs:subClassOf :MiscTrait .


:MoveMechanic rdfs:subClassOf :Characteristic .
:swim a :MoveMechanic .
:burrow a :MoveMechanic .
:incorporealMovement a :MoveMechanic;
    rdfs:label "Movement as an incorporeal creature";
    rdfs:comment "This creature can enter or pass through solid objects, but must remain adjacent to the objectâ€™s exterior, and so cannot pass entirely through an object whose space is larger than its own. It can sense the presence of creatures or objects within a square adjacent to its current location, but enemies have total concealment (50% miss chance) from an incorporeal creature that is inside an object. In order to see farther from the object it is in and attack normally, the incorporeal creature must emerge. An incorporeal creature inside an object has total cover, but when it attacks a creature outside the object it only has cover, so a creature outside with a readied action could strike at it as it attacks. An incorporeal creature cannot pass through a force effect.";
.
:ground a :MoveMechanic;
    rdfs:comment "The creature's movement on the ground.";
.

:Fly rdfs:subClassOf :MoveMechanic .
:perfectFlight a :Fly;
    rdfs:label "Perfect Flight";
.
:flight a :Fly
.

:AbilityScore rdfs:subClassOf :Characteristic .
:Str 
    rdfs:subClassOf :AbilityScore ;
.
:Dex 
    rdfs:subClassOf :AbilityScore ;
.
:Con 
    rdfs:subClassOf :AbilityScore ;
.
:Int 
    rdfs:subClassOf :AbilityScore ;
.
:Wis 
    rdfs:subClassOf :AbilityScore ;
.
:Cha 
    rdfs:subClassOf :AbilityScore ;
.


:ExistentialStatus rdfs:subClassOf :Characteristic .
:native a :ExistentialStatus;
    rdfs:comment "Creature is currently on its native plane.";
.
:nonNative a :ExistentialStatus;
    rdfs:label "Non-Native";
    rdfs:comment "Creature is not currently on its native plane.";
.

:ShapeChangeStatus rdfs:subClassOf :Characteristic .
:asHumanoid a :ShapeChangeStatus;
    rdfs:label "As Humanoid";
    rdfs:comment "Creature is currently in humanoid form.";
.

:Size rdfs:subClassOf :Characteristic .
:fine a :Size .
:diminutive a :Size .
:tiny a :Size .
:small a :Size .
:medium a :Size .
:large a :Size .
:huge a :Size .
:gargantuan a :Size .
:colossal a :Size .
:colossalPlus a :Size .


:SpecialAction rdfs:subClassOf :Characteristic .

:SpecialArmorClass rdfs:subClassOf :Characteristic .

:SupernaturalAbility
    rdfs:subClassOf :Characteristic;
    rdfs:comment "Supernatural ability; its use draws no attack of opportunity, it cannot be dispelled, but it can be blocked with an antimagic field."
.

:ExtraordinaryAbility
    rdfs:subClassOf :Characteristic;
    rdfs:comment "Extraordinary (non-magical) ability; its use draws no attack of opportunity, and it cannot be dispelled or otherwise interfered with by any anti-magic means."
.

:SpellLikeAbility 
    rdfs:subClassOf :Characteristic;
    rdfs:comment "Spell-like ability; its use can be interfered with using dispel, spell resistance, and antimagic; its use incurs attacks of opportunity."
.

:Aura
    rdfs:subClassOf :Characteristic;
    rdfs:comment "Permanent effect that extends some distance around the body of the creature.";
.

:AttackGroup
    rdfs:subClassOf :Characteristic;
    rdfs:comment "A group of attacks which may all be executed in the same round.";
.
:PhysicalAttack rdfs:subClassOf :Characteristic .
:MeleeAttack rdfs:subClassOf :PhysicalAttack .
:bite a :MeleeAttack .
:claw a :MeleeAttack .
:wing a :MeleeAttack .
:tail a :MeleeAttack .

:RangedAttack rdfs:subClassOf :PhysicalAttack .

:TouchAttack rdfs:subClassOf :Characteristic.

:AttackOption rdfs:subClassOf :Characteristic;
    rdfs:comment "A special attack possessed by a creature, or a modifier to a regular attack";
.

:RetryableSkill 
    rdfs:subClassOf :Characteristic ;
    rdfs:comment "If skill attempt fails, another attempt may be made.";
.
:PsionicSkill
    rdfs:subClassOf :Characteristic ;
    rdfs:comment "Skill is psionic in nature." ;
.
:RequiresRanks
    rdfs:subClassOf :Characteristic ;
    rdfs:comment "Skill may not be used untrained, i.e., without ranks.";
.
:ArmorCheckPenalty
    rdfs:subClassOf :Characteristic ;
    rdfs:comment "Some penalty will apply to this skill check depending on the armor the character is wearing.";
.
:SubSkill rdfs:subClassOf :Characteristic .
:Skill rdfs:subClassOf :Characteristic .
:MonsterHasSkill a rdfs:Class;
    rdfs:comment "The skill of a particular monster.".


:SkillSynergy rdfs:subClassOf :Characteristic .

:Feat rdfs:subClassOf :Characteristic .
:FeatType rdfs:subClassOf :Characteristic .
:PsionicFeat a :FeatType;
    rdfs:label "Psionic"
.
:DivineFeat a :FeatType;
    rdfs:label "Divine"
.
:EpicFeat a :FeatType;
    rdfs:label "Epic"
.
:GeneralFeat a :FeatType;
    rdfs:label "General"
.
:WildFeat a :FeatType;
    rdfs:label "Wild"
.
:MetamagicFeat a :FeatType;
    rdfs:label "Metamagic"
.
:FighterFeat a :FeatType;
    rdfs:label "Fighter"
.
:ItemCreationFeat a :FeatType;
    rdfs:label "Item Creation"
.
:MetapsionicFeat a :FeatType;
    rdfs:label "Metapsionic"
.
:CanTakeMultipleFeat 
    rdfs:subClassOf :Characteristic;
    rdfs:comment "This feat may be taken more than once";
.
:StackableFeat
    rdfs:subClassOf :Characteristic;
    rdfs:comment "When this feat is taken more than once, its effects stack";
.
:ArmorClassFeat a rdfs:Class;
    rdfs:comment "Should appear in statblocks near the armor class stat" .
:SpecialActionFeat a rdfs:Class;
    rdfs:comment "Should appear in statblocks near the special actions" .
:SpeedFeat a rdfs:Class;
    rdfs:comment "Should appear in statblocks near the speed stat" .
:AttackOptionFeat a rdfs:Class;
    rdfs:comment "Should appear in statblocks near the attacks" .
:RangedAttackFeat a rdfs:Class;
    rdfs:comment "Should appear in statblocks near the ranged attacks" .
:MonsterBonusFeat a rdfs:Class;
    rdfs:comment "Feat always possessed by a monster even when it does not actually satisfy the requirements" .
:MonsterHasFeat a rdfs:Class;
    rdfs:comment "The feat of a particular monster.".  


:Armor
    rdfs:subClassOf :Characteristic;
    rdfs:comment "Item is a type of armor";
.
:Weapon
    rdfs:subClassOf :Characteristic;
    rdfs:comment "Item is a weapon";
.
:ExoticWeapon rdfs:subClassOf :Characteristic .
:MartialWeapon rdfs:subClassOf :Characteristic .
:NaturalWeapon rdfs:subClassOf :Characteristic .
:Crossbow rdfs:subClassOf :Characteristic .

:SpellSchool rdfs:subClassOf :Characteristic .
:SpellDomain rdfs:subClassOf :Characteristic .
:PsionicPower rdfs:subClassOf :Characteristic .

:WornItemLocation rdfs:subClassOf :Characteristic .
:headLocation a :WornItemLocation;
    rdfs:label "On the head";
    rdfs:comment "A headband, hat, or helmet may be worn here.";
.
:eyesLocation a :WornItemLocation;
    rdfs:label "On the eyes";
    rdfs:comment "One pair of eye lenses or goggles may be worn here.";
.
:shouldersLocation a :WornItemLocation;
    rdfs:label "Around the shoulders";
    rdfs:comment "One cloak, cape, or mantle may be worn here.";
.
:wrapAroundLocation a :WornItemLocation;
    rdfs:label "Wrapped around the entire body";
    rdfs:comment "One robe may be worn here.";
.
:neckOrPinLocation a :WornItemLocation;
    rdfs:label "On the neck or pinned to the chest";
    rdfs:comment "One amulet, brooch, medallion, necklace, periapt, or scarab may be worn here.";
.
:wholeBodyLocation a :WornItemLocation;
    rdfs:label "Covering most of the body";
    rdfs:comment "One suit of armor may be worn here.";
.
:torsoLocation a :WornItemLocation;
    rdfs:label "Covering the upper torso";
    rdfs:comment "One vest, vestment, or shirt may be worn here.";
.
:wristLocation a :WornItemLocation;
    rdfs:label "On the wrists";
    rdfs:comment "One pair of bracers or bracelets may be worn here.";
.
:handLocation a :WornItemLocation;
    rdfs:label "On the hands";
    rdfs:comment "One pair of gloves or gauntlets may be worn here.";
.
:fingerLocation a :WornItemLocation;
    rdfs:label "On the finger";
    rdfs:comment "One ring may be worn here (to a maximum of--usually--two)";
.
:waistLocation a :WornItemLocation;
    rdfs:label "Around the waist";
    rdfs:comment "One belt may be worn here";
.
:feetLocation a :WornItemLocation;
    rdfs:label "On the feet";
    rdfs:comment "One pair of boots may be worn here";
.

:Spell rdfs:subClassOf :Characteristic .
:ArcaneSpell rdfs:subClassOf :Characteristic .
:DivineSpell rdfs:subClassOf :Characteristic .
:SpellTargetYou rdfs:subClassOf :Characteristic ;
    rdfs:label "You";
    rdfs:comment "The caster himself is the target";
.
:AreaEffectSpell rdfs:subClassOf :Characteristic .

:MagicItemMaterial rdfs:subClassOf :Characteristic .
:adamantine a :MagicItemMaterial .
:darkwood a :MagicItemMaterial .
:dragonhide a :MagicItemMaterial .
:mithral a :MagicItemMaterial .
:alchemicalSilver a :MagicItemMaterial .
:coldIron a :MagicItemMaterial .

:SpellLikeAbility a :Characteristic .

:Familiar a :Characteristic;
    rdfs:comment "A creature which is an arcane familiar.";
.

:ReferentCharacter a rdfs:Class;
    rdfs:comment "The individual being referred to by the statement";
.

:SpellOrSpellLikeAbility a rdfs:Class;
    rdfs:comment "Either a spell or a spell-like ability; something castable";
.

:SpellLevel a rdfs:Class .
:spellLevel1 a :SpellLevel .
:spellLevel2 a :SpellLevel .
:spellLevel3 a :SpellLevel .
:spellLevel4 a :SpellLevel .
:spellLevel5 a :SpellLevel .
:spellLevel6 a :SpellLevel .
:spellLevel7 a :SpellLevel .
:spellLevel8 a :SpellLevel .
:spellLevel9 a :SpellLevel .



:Monster rdfs:subClassOf :Characteristic .

:TreasureValue rdfs:subClassOf :Characteristic .
:standardTreasure a :TreasureValue .
:doubleStandardTreasure a :TreasureValue .
:tripleStandardTreasure a :TreasureValue .
:noTreasure a :TreasureValue .
:asCharacter a :TreasureValue .
:halfStandard a :TreasureValue .

:TreasureType rdfs:subClassOf :Characteristic .
:Coins rdfs:subClassOf :TreasureType .
:Goods rdfs:subClassOf :TreasureType .
:Items rdfs:subClassOf :TreasureType .

:AttackForm a rdfs:Class;
    rdfs:comment "One weapon a monster can use, possibly multiple times in a round, to attack.";  
.

:ArmorValue rdfs:subClassOf :Characteristic;
        rdfs:comment "A value that goes into a monster's total armor, such as a shield or insight";
.
